src/travorder/Next.v
@@ -1,0 +1,191 @@
+From hahn Require Import Hahn.
+
+From imm Require Import AuxDef Events Execution.
+From imm Require Import Execution_eco imm_s_hb imm_s imm_bob.
+From imm Require Import imm_s_ppo CombRelations.
+From imm Require Import imm_s_rfppo.
+From imm Require Import FinExecution.
+
+From imm Require Import TraversalOrder.
+From imm Require Import TLSCoherency.
+From imm Require Import IordCoherency.
+From imm Require Import SimClosure.
+Require Import TlsEventSets.
+Require Import EventsTraversalOrder.
+
+Section Next.
+  Variable G : execution.
+  Variable WF : Wf G.
+  Variable COM : complete G.
+  Variable sc : relation actid.
+  Variable IMMCON : imm_consistent G sc.
+
+  Notation "'sb'" := (sb G).
+  Notation "'rmw'" := (rmw G).
+  Notation "'data'" := (data G).
+  Notation "'addr'" := (addr G).
+  Notation "'ctrl'" := (ctrl G).
+  Notation "'rf'" := (rf G).
+  Notation "'co'" := (co G).
+  Notation "'coe'" := (coe G).
+  Notation "'fr'" := (fr G).
+
+  Notation "'eco'" := (eco G).
+
+  Notation "'bob'" := (bob G).
+  Notation "'fwbob'" := (fwbob G).
+  Notation "'ppo'" := (ppo G).
+  Notation "'fre'" := (fre G).
+  Notation "'rfi'" := (rfi G).
+  Notation "'rfe'" := (rfe G).
+  Notation "'deps'" := (deps G).
+  Notation "'detour'" := (detour G).
+  Notation "'release'" := (release G).
+  Notation "'sw'" := (sw G).
+  Notation "'hb'" := (hb G).
+
+  Notation "'ar'" := (ar G sc).
+
+  Notation "'urr'" := (urr G sc).
+  Notation "'c_acq'" := (c_acq G sc).
+  Notation "'c_cur'" := (c_cur G sc).
+  Notation "'c_rel'" := (c_rel G sc).
+  Notation "'t_acq'" := (t_acq G sc).
+  Notation "'t_cur'" := (t_cur G sc).
+  Notation "'t_rel'" := (t_rel G sc).
+  Notation "'S_tm'" := (S_tm G).
+  Notation "'S_tmr'" := (S_tmr G).
+  Notation "'msg_rel'" := (msg_rel G sc).
+
+Notation "'lab'" := (lab G).
+Notation "'loc'" := (loc lab).
+Notation "'val'" := (val lab).
+Notation "'mod'" := (Events.mod lab).
+Notation "'same_loc'" := (same_loc lab).
+
+Notation "'E'" := (acts_set G).
+Notation "'R'" := (fun x => is_true (is_r lab x)).
+Notation "'W'" := (fun x => is_true (is_w lab x)).
+Notation "'F'" := (fun x => is_true (is_f lab x)).
+Notation "'RW'" := (R ∪₁ W).
+Notation "'FR'" := (F ∪₁ R).
+Notation "'FW'" := (F ∪₁ W).
+Notation "'R_ex'" := (fun a => is_true (R_ex lab a)).
+Notation "'W_ex'" := (W_ex G).
+Notation "'W_ex_acq'" := (W_ex ∩₁ (fun a => is_true (is_xacq lab a))).
+
+Notation "'Init'" := (fun a => is_true (is_init a)).
+Notation "'Loc_' l" := (fun x => loc x = Some l) (at level 1).
+Notation "'Tid_' t" := (fun x => tid x = t) (at level 1).
+Notation "'W_' l" := (W ∩₁ Loc_ l) (at level 1).
+
+Definition next C := E ∩₁ dom_cond sb C ∩₁ set_compl C.
+  
+Lemma next_helper C a 
+  (IC : is_init ∩₁ E ⊆₁ C)
+  (CE : C ⊆₁ E)
+  (CC : C ⊆₁ dom_cond sb C)
+  (NEXT: next C a) :
+  ⦗Tid_ (tid a) ∪₁ Init⦘ ⨾ ⦗C⦘ ≡ ⦗dom_rel (sb ⨾ ⦗eq a⦘)⦘.
+Proof using WF.
+split.
+- unfolder; ins; desc; splits; eauto; eexists; splits; eauto; subst.
+  assert (~ is_init a) as NA.
+  { intros H; apply NEXT, IC. split; auto.
+    apply NEXT. }
+  assert (E y) as EY.
+    by apply CE.
+  assert (E a) as EA.
+    by apply NEXT.
+  desf; [|by apply init_ninit_sb].
+  symmetry in H0.
+  eapply same_thread in H0; eauto.
+  desf. exfalso. red in H0; desf; [by apply NEXT in H1|].
+  apply NEXT.
+  apply CC in H1.
+  apply H1; basic_solver 8.
+- rewrite sb_tid_init'.
+  unfold same_tid; unfolder; ins; desf; splits; eauto.
+  apply NEXT; basic_solver 10.
+apply IC. split; auto.
+apply (dom_l (@wf_sbE G)) in H2.
+apply seq_eqv_l in H2. desf.
+Qed.
+
+
+Lemma next_helper' a T
+      (TCOH : tls_coherent G T)
+      (ICOH : iord_coherent G sc T)
+  (NEXT: next (covered T) a) :
+  ⦗Tid_ (tid a) ∪₁ Init⦘ ⨾ ⦗covered T⦘ ≡ ⦗dom_rel (sb ⨾ ⦗eq a⦘)⦘.
+Proof using WF IMMCON.
+  apply next_helper; auto using init_covered, coveredE.
+  apply dom_rel_to_cond. eapply dom_sb_covered; eauto.  
+Qed.
+
+  Lemma next_n_init T e
+        (NEXT : next (covered T) e)
+        (TCOH: tls_coherent G T):
+    ~ Init e.
+  Proof using.
+    intros HH. apply NEXT.
+    eapply init_covered; eauto. split; auto.
+    apply NEXT.
+  Qed.
+
+  Lemma issuable_next_w T 
+    (TCOH: tls_coherent G T)
+    (ICOH: iord_coherent G sc T):
+    W ∩₁ next (covered T) ⊆₁ issuable G sc T.
+  Proof using WF IMMCON.
+    unfold issuable, next.
+    apply set_subset_inter_r; split.
+    { basic_solver 10. }
+    rewrite !set_interA.
+    arewrite (dom_cond sb (covered T) ∩₁ set_compl (covered T) ⊆₁ dom_cond sb (covered T)).
+    { basic_solver 10. }
+    rewrite !dom_cond_alt. rewrite <- !set_bunion_inter_compat_l.
+    apply set_subset_bunion_l. ins.
+    rewrite <- !set_bunion_inter_compat_r. rewrite set_collect_bunion.
+    apply set_subset_bunion_r with (a := mkTL ta_issue x).
+    2: { unfolder. ins. desc. eexists. splits; vauto. }
+
+    filter_iord_seq.
+    rewrite <- id_inter, set_inter_absorb_l; [| basic_solver].
+    rewrite inclusion_restr. rewrite dom_union. apply set_subset_union_l. split.
+    { assert (T ∩₁ action ↓₁ eq ta_cover ⊆₁ T) as <-; [basic_solver| ].
+      apply dom_rel_collect_event2; [basic_solver| ].
+      rewrite <- COND. rewrite fwbob_in_sb. basic_solver. } 
+    assert (T ∩₁ action ↓₁ eq ta_issue ⊆₁ T) as <-; [basic_solver| ].
+    apply dom_rel_collect_event2; [basic_solver| ].
+    rewrite event_collect_eq. 
+    
+    rewrite ct_end, !seqA.
+    arewrite (ar ∪ rf ⨾ ppo ∩ same_loc ⊆ (ar ∪ sb)^? ⨾ ar) at 2.
+    { apply inclusion_union_l; [basic_solver|].
+      rewrite rfi_union_rfe. rewrite rfe_in_ar, ppo_in_ar.
+      arewrite (rfi ⊆ sb). basic_solver 10. }
+    arewrite (ar ⨾ ⦗W⦘ ⊆ sb).
+    { unfold imm_s.ar.
+      rewrite !seq_union_l. rewrite (ar_int_in_sb WF).
+      rewrite wf_scD with (sc:=sc); [|by apply IMMCON].
+      rewrite (wf_rfeD WF). type_solver. }    
+    apply dom_rel_helper_in in COND. rewrite COND.
+    arewrite ((ar ∪ sb)^? ⨾ ⦗covered T⦘ ⊆ ⦗covered T ∪₁ issued T⦘ ⨾ (ar ∪ sb)^? ⨾ ⦗covered T⦘).
+    2: { etransitivity.
+         2: apply ar_rf_ppo_loc_rt_CI_in_I; eauto.
+         { basic_solver 20. }
+         apply IMMCON. }
+    apply dom_rel_helper_in.
+    rewrite crE, !seq_union_l, !dom_union, seq_id_l.
+    unionL; [basic_solver| |].
+    2: { rewrite dom_sb_covered; basic_solver. }
+    apply ar_C_in_CI; eauto. apply IMMCON.
+  Qed. 
+
+End Next. 
+
+Global Add Parametric Morphism : next with signature
+       eq ==> (@set_equiv actid) ==> (@set_equiv actid) as next_more. 
+Proof using. ins. unfold next. rewrite H. basic_solver. Qed. 
+
