src/travorder/ReserveClos.v
@@ -1,0 +1,123 @@
+Require Import Lia.
+From hahn Require Import Hahn.
+Require Import AuxRel2.
+Require Import AuxDef.
+Require Import Events.
+Require Import Execution.
+Require Import imm_s.
+Require Import TlsEventSets.
+Require Import TraversalOrder.
+Require Import TLSCoherency.
+Require Import IordCoherency.
+
+(* Require Import Prog. *)
+(* Require Import ProgToExecution. *)
+(* Require Import imm_s_ppo. *)
+(* Require Import CombRelations. *)
+(* Require Import ProgToExecutionProperties. *)
+(* Require Import RMWinstrProps. *)
+(* Require Import FairExecution. *)
+(* Require Import FinExecution. *)
+(* Require Import FinThreads. *)
+
+(* Require Import ImmFair.  *)
+
+(* Require Import SimTraversal. *)
+(* Require Import SimTraversalProperties. *)
+(* Require Import TraversalConfigAlt. *)
+(* Require Import SetSize. *)
+(* Require Import SimClosure. *)
+
+(* Require Import TlsAux2. *)
+(* Require Import SimIordTraversal. *)
+(* Require Import EventsTraversalOrder. *)
+
+Set Implicit Arguments.
+
+Section ReserveClos.
+Definition reserve_clos tc := tc ∪₁ eq ta_reserve <*> (issued tc).
+
+Global Add Parametric Morphism : reserve_clos with signature
+    set_subset ==> set_subset as reserve_clos_mori.
+Proof using.
+  intros x y HH. unfold reserve_clos. rewrite HH.
+  clear. basic_solver.
+Qed. 
+
+Global Add Parametric Morphism : reserve_clos with signature
+    set_equiv ==> set_equiv as reserve_clos_more.
+Proof using.
+  intros x y [HH AA]. split.
+  { now rewrite HH. }
+  now rewrite AA.
+Qed. 
+
+Lemma reserve_clos_union s s' :
+  reserve_clos (s ∪₁ s') ≡₁ reserve_clos s ∪₁ reserve_clos s'.
+Proof using.
+  unfold reserve_clos.
+  rewrite !issued_union.
+  rewrite set_pair_union_r.
+  clear. basic_solver 10.
+Qed.
+
+Variable G : execution.
+Variable sc : relation actid.
+Hypothesis WF : Wf G.
+Hypothesis WFSC : wf_sc G sc.
+Notation "'E'" := (acts_set G).
+Notation "'W'" := (fun x => is_true (is_w (lab G) x)).
+
+Lemma reserve_clos_iord_coherent tc
+  (ICOH : iord_coherent G sc tc) :
+  iord_coherent G sc (reserve_clos tc).
+Proof using.
+  unfold reserve_clos.
+  red. rewrite id_union, seq_union_r, dom_union.
+  unionL.
+  { now unionR left. }
+  transitivity (@set_empty trav_label).
+  2: clear; basic_solver.
+  rewrite iord_no_reserve.
+  unfold set_pair.
+  unfolder. ins. do 2 desf.
+Qed.
+
+Lemma covered_reserve_clos tc : covered (reserve_clos tc) ≡₁ covered tc.
+Proof using.
+  ins. unfold reserve_clos. rewrite covered_union, covered_ta_reserve.
+  now rewrite set_union_empty_r.
+Qed.
+
+Lemma issued_reserve_clos tc : issued (reserve_clos tc) ≡₁ issued tc.
+Proof using.
+  ins. unfold reserve_clos. rewrite issued_union, issued_ta_reserve.
+  now rewrite set_union_empty_r.
+Qed.
+
+Lemma reserved_reserve_clos tc : reserved (reserve_clos tc) ≡₁ reserved tc ∪₁ issued tc.
+Proof using.
+  ins. unfold reserve_clos.
+  now rewrite reserved_union, reserved_ta_reserve.
+Qed.
+
+Lemma reserve_clos_eq_ta_cover w : reserve_clos (eq (ta_cover, w)) ≡₁ eq (ta_cover, w).
+Proof using.
+  ins. unfold reserve_clos. rewrite issued_eq_ta_cover.
+  unfold set_pair. unfolder. split; ins; do 2 desf; eauto.
+Qed.
+
+Lemma reserve_clos_eq_ta_issue w : reserve_clos (eq (ta_issue, w)) ≡₁ eq (ta_issue, w) ∪₁ eq (ta_reserve, w).
+Proof using.
+  ins. unfold reserve_clos. rewrite issued_singleton.
+  apply set_union_more; eauto with hahn.
+  now rewrite set_pair_exact.
+Qed.
+
+Lemma reserve_clos_eq_ta_reserve w : reserve_clos (eq (ta_reserve, w)) ≡₁ eq (ta_reserve, w).
+Proof using.
+  ins. unfold reserve_clos. rewrite issued_eq_ta_reserve.
+  unfold set_pair. unfolder. split; ins; do 2 desf; eauto.
+Qed.
+
+End ReserveClos.
