src/travorder/TlsAux2.v
@@ -1,0 +1,56 @@
+From hahn Require Import Hahn.
+
+From imm Require Import AuxDef Events Execution.
+From imm Require Import Execution_eco imm_s_hb imm_s imm_bob.
+From imm Require Import imm_s_ppo CombRelations.
+From imm Require Import imm_s_rfppo.
+From imm Require Import FinExecution.
+
+From imm Require Import TraversalOrder.
+From imm Require Import TLSCoherency.
+From imm Require Import IordCoherency.
+
+From imm Require Import AuxRel2.
+
+Set Implicit Arguments.
+
+Section TLSCoherentMore.
+Context G G'
+        (EQACTS : acts_set    G' ≡₁ acts_set    G)
+        (EQTIDS : threads_set G' ≡₁ threads_set G)
+        (EQW    : is_w (lab G')  ≡₁ is_w (lab G))
+        T
+        (TCOH   : tls_coherent G T).
+
+Lemma is_ta_propagate_to_G_more :
+  is_ta_propagate_to_G G' ≡₁ is_ta_propagate_to_G G.
+Proof using EQTIDS.
+  unfold is_ta_propagate_to_G.
+  now rewrite EQTIDS.
+Qed.
+
+Lemma init_tls_more : init_tls G' ≡₁ init_tls G.
+Proof using EQACTS EQTIDS.
+  unfold init_tls.
+  apply set_pair_more.
+  2: now rewrite EQACTS.
+  now rewrite is_ta_propagate_to_G_more.
+Qed.
+
+Lemma exec_tls_more : exec_tls G' ≡₁ exec_tls G.
+Proof using EQACTS EQTIDS EQW.
+  unfold exec_tls.
+  rewrite EQACTS.
+  rewrite is_ta_propagate_to_G_more.
+  now rewrite EQW.
+Qed.
+
+Lemma tls_coherent_more : tls_coherent G' T.
+Proof using EQACTS EQTIDS EQW TCOH.
+  destruct TCOH as [AA BB].
+  constructor.
+  all: rewrite init_tls_more; auto.
+  rewrite exec_tls_more; auto.
+Qed.
+
+End TLSCoherentMore.
