src/travorder/TlsEventSets.v
@@ -1,0 +1,542 @@
+From hahn Require Import Hahn.
+Require Import TraversalOrder.
+Require Import TLSCoherency.
+Require Import IordCoherency.
+Require Import Events.
+Require Import Execution.
+Require Import AuxRel.
+Require Import AuxDef.
+Require Import imm_s.
+
+Set Implicit Arguments.
+
+Definition issued   tc := event ↑₁ (tc ∩₁ action ↓₁ (eq ta_issue)).
+Definition covered  tc := event ↑₁ (tc ∩₁ action ↓₁ (eq ta_cover)).
+Definition reserved tc := event ↑₁ (tc ∩₁ action ↓₁ (eq ta_reserve)).
+
+Definition propagated G TLS :=
+  event ↑₁ (TLS ∩₁ (action ↓₁ is_ta_propagate_to_G G)). 
+Definition propagated_thread TLS t := 
+  event ↑₁ (TLS ∩₁ (action ↓₁ eq (ta_propagate t))). 
+
+Definition coverable G sc T :=
+  acts_set G ∩₁ event ↑₁ (dom_cond (iord G sc) T ∩₁ action ↓₁ eq ta_cover). 
+Definition issuable G sc T :=
+  acts_set G ∩₁ (is_w (lab G)) ∩₁ event ↑₁ (dom_cond (iord G sc) T ∩₁ action ↓₁ eq ta_issue). 
+
+
+Lemma tls_set_alt T a e:
+  (event ↑₁ (T ∩₁ action ↓₁ eq a)) e <-> T (mkTL a e). 
+Proof using. 
+  unfolder. split; ins; desc; eauto.
+  destruct y; ins; by subst. 
+Qed. 
+
+Lemma propagated_alt G T: 
+  propagated G T ≡₁ ⋃₁ t ∈ threads_set G \₁ eq tid_init, propagated_thread T t.
+Proof using.
+  unfold propagated_thread, propagated, is_ta_propagate_to_G. basic_solver 10.
+Qed.   
+
+Lemma covered_single e:
+  covered (eq (mkTL ta_cover e)) ≡₁ eq e. 
+Proof using.
+  unfold covered. rewrite set_inter_absorb_r; basic_solver.
+Qed.
+
+Lemma reserved_ta_reserve s :
+  reserved (eq ta_reserve <*> s) ≡₁ s.
+Proof using.
+  unfold reserved.
+  unfolder; split; ins; desf.
+  { destruct y; ins. desf. }
+  eexists (_, _). splits; ins; eauto.
+Qed.
+
+Lemma issued_ta_reserve s :
+  issued (eq ta_reserve <*> s) ≡₁ ∅.
+Proof using.
+  unfold issued.
+  unfolder; split; ins; desf.
+  destruct y; ins. desf.
+Qed.
+
+Lemma covered_ta_reserve s :
+  covered (eq ta_reserve <*> s) ≡₁ ∅.
+Proof using.
+  unfold covered.
+  unfolder; split; ins; desf.
+  destruct y; ins. desf.
+Qed.
+
+Lemma issued_eq_ta_cover w : issued (eq (ta_cover, w)) ≡₁ ∅.
+Proof using.
+  unfold issued. clear. basic_solver 10.
+Qed.
+
+Lemma covered_eq_ta_issue w : covered (eq (ta_issue, w)) ≡₁ ∅.
+Proof using.
+  unfold covered. clear. basic_solver 10.
+Qed.
+
+Lemma covered_eq_ta_reserve w : covered (eq (ta_reserve, w)) ≡₁ ∅.
+Proof using.
+  unfold covered. clear. basic_solver 10.
+Qed.
+
+Lemma issued_eq_ta_reserve w : issued (eq (ta_reserve, w)) ≡₁ ∅.
+Proof using.
+  unfold issued. clear. basic_solver 10.
+Qed.
+
+Lemma reserved_eq_ta_issue w : reserved (eq (ta_issue, w)) ≡₁ ∅.
+Proof using.
+  unfold reserved. clear. basic_solver 10.
+Qed.
+
+Lemma reserved_eq_ta_cover w : reserved (eq (ta_cover, w)) ≡₁ ∅.
+Proof using.
+  unfold reserved. clear. basic_solver 10.
+Qed.
+
+Section MorphismsCIRP.
+
+Local Ltac cirp_morph :=
+  intros x y HH; unfold covered, issued, reserved, propagated;
+  solve [now rewrite HH|now rewrite <- HH].
+
+Global Add Parametric Morphism : covered with signature
+    (@set_subset trav_label) ==> (@set_subset actid)
+       as covered_mori.
+Proof using. cirp_morph. Qed.
+
+Global Add Parametric Morphism : issued with signature
+    (@set_subset trav_label) ==> (@set_subset actid)
+       as issued_mori.
+Proof using. cirp_morph. Qed.
+
+Global Add Parametric Morphism : reserved with signature
+    (@set_subset trav_label) ==> (@set_subset actid)
+       as reserved_mori.
+Proof using. cirp_morph. Qed.
+
+Global Add Parametric Morphism : propagated with signature
+    eq ==> (@set_subset trav_label) ==> (@set_subset actid)
+       as propagated_mori.
+Proof using. intros G. cirp_morph. Qed. 
+
+Global Add Parametric Morphism : covered with signature
+    (@set_equiv trav_label) ==> (@set_equiv actid)
+       as covered_more.
+Proof using. cirp_morph. Qed.
+
+Global Add Parametric Morphism : issued with signature
+    (@set_equiv trav_label) ==> (@set_equiv actid)
+       as issued_more.
+Proof using. cirp_morph. Qed. 
+
+Global Add Parametric Morphism : reserved with signature
+    (@set_equiv trav_label) ==> (@set_equiv actid)
+       as reserved_more.
+Proof using. cirp_morph. Qed. 
+
+Global Add Parametric Morphism : propagated with signature
+    eq ==> (@set_equiv trav_label) ==> (@set_equiv actid)
+       as propagated_more.
+Proof using. intros G. cirp_morph. Qed. 
+
+End MorphismsCIRP. 
+
+Section SimplificationsCIRP. 
+
+
+Lemma tls_set_inter_helper T1 T2 (a: trav_action):
+  event ↑₁ ((T1 ∩₁ T2) ∩₁ action ↓₁ eq a) ≡₁
+  event ↑₁ (T1 ∩₁ action ↓₁ eq a) ∩₁ event ↑₁ (T2 ∩₁ action ↓₁ eq a).
+Proof using. 
+  split; try basic_solver 10.
+  unfolder. ins. desc. destruct y, y0; ins; subst. eauto. 
+Qed.  
+
+Lemma tls_set_minus_helper T1 T2 (a: trav_action):
+  event ↑₁ ((T1 \₁ T2) ∩₁ action ↓₁ eq a) ≡₁
+  event ↑₁ (T1 ∩₁ action ↓₁ eq a) \₁ event ↑₁ (T2 ∩₁ action ↓₁ eq a).
+Proof using.
+  split; try basic_solver 10.
+  unfolder. ins. desc. destruct y; ins; subst. 
+  splits; try by eauto.
+  intro. desc. ins. desc. destruct y; ins; subst. done. 
+Qed.
+
+Lemma covered_events (A: actid -> Prop): covered (event ↓₁ A) ⊆₁ A. 
+Proof using. unfold covered. basic_solver. Qed. 
+
+Lemma issued_events (A: actid -> Prop): issued (event ↓₁ A) ⊆₁ A. 
+Proof using. unfold issued. basic_solver. Qed. 
+
+Lemma reserved_events (A: actid -> Prop): reserved (event ↓₁ A) ⊆₁ A. 
+Proof using. unfold reserved. basic_solver. Qed. 
+
+Lemma propagated_events G (A: actid -> Prop): propagated G (event ↓₁ A) ⊆₁ A. 
+Proof using. unfold propagated. basic_solver. Qed. 
+
+Lemma covered_union T1 T2: covered (T1 ∪₁ T2) ≡₁ covered T1 ∪₁ covered T2. 
+Proof using. unfold covered. basic_solver 10. Qed. 
+Lemma covered_inter T1 T2: covered (T1 ∩₁ T2) ≡₁ covered T1 ∩₁ covered T2.
+Proof using. apply tls_set_inter_helper. Qed.  
+Lemma covered_minus T1 T2: covered (T1 \₁ T2) ≡₁ covered T1 \₁ covered T2.
+Proof using. apply tls_set_minus_helper. Qed. 
+
+Lemma issued_union T1 T2: issued (T1 ∪₁ T2) ≡₁ issued T1 ∪₁ issued T2. 
+Proof using. unfold issued. basic_solver 10. Qed. 
+Lemma issued_inter T1 T2: issued (T1 ∩₁ T2) ≡₁ issued T1 ∩₁ issued T2.
+Proof using. apply tls_set_inter_helper. Qed.  
+Lemma issued_minus T1 T2: issued (T1 \₁ T2) ≡₁ issued T1 \₁ issued T2.
+Proof using. apply tls_set_minus_helper. Qed. 
+
+Lemma reserved_union T1 T2: reserved (T1 ∪₁ T2) ≡₁ reserved T1 ∪₁ reserved T2. 
+Proof using. unfold reserved. basic_solver 10. Qed. 
+Lemma reserved_inter T1 T2: reserved (T1 ∩₁ T2) ≡₁ reserved T1 ∩₁ reserved T2.
+Proof using. apply tls_set_inter_helper. Qed.  
+Lemma reserved_minus T1 T2: reserved (T1 \₁ T2) ≡₁ reserved T1 \₁ reserved T2.
+Proof using. apply tls_set_minus_helper. Qed. 
+
+Lemma propagated_union G T1 T2:
+  propagated G (T1 ∪₁ T2) ≡₁ propagated G T1 ∪₁ propagated G T2. 
+Proof using. unfold propagated. basic_solver 10. Qed.
+(* Not true: an event can be propagated into different threads in T1 and T2*)
+(* Lemma propagated_inter G T1 T2: *)
+(*   propagated G (T1 ∩₁ T2) ≡₁ propagated G T1 ∩₁ propagated G T2.  *)
+(* Lemma propagated_minus G T1 T2: *)
+(*   propagated G (T1 \₁ T2) ≡₁ propagated G T1 \₁ propagated G T2. *)
+
+Lemma covered_singleton e:
+  covered (eq (mkTL ta_cover e)) ≡₁ eq e.
+Proof using. unfold covered. split; basic_solver. Qed. 
+
+Lemma issued_singleton e:
+  issued (eq (mkTL ta_issue e)) ≡₁ eq e.
+Proof using. unfold issued. split; basic_solver. Qed. 
+
+Lemma reserved_singleton e:
+  reserved (eq (mkTL ta_reserve e)) ≡₁ eq e.
+Proof using. unfold reserved. split; basic_solver. Qed. 
+
+(* TODO: find the correct statement and premises *)
+(* Lemma propagated_singleton G t e : *)
+(*   propagated G (eq (mkTL (ta_propagate t) e)) ≡₁ eq e. *)
+
+Lemma covered_noncover_empty S
+      (NONCOVER: set_disjoint S (action ↓₁ eq ta_cover)):
+  covered S ≡₁ ∅.
+Proof using. unfold covered. split; basic_solver. Qed. 
+
+Lemma issued_nonissue_empty S
+      (NONISSUE: set_disjoint S (action ↓₁ eq ta_issue)):
+  issued S ≡₁ ∅.
+Proof using. unfold issued. split; basic_solver. Qed. 
+
+Lemma reserved_nonreserve_empty S
+      (NONISSUE: set_disjoint S (action ↓₁ eq ta_reserve)):
+  reserved S ≡₁ ∅.
+Proof using. unfold reserved. split; basic_solver. Qed. 
+
+Lemma propagated_nonpropagated_empty G S
+      (NONPROP: set_disjoint S (action ↓₁ is_ta_propagate_to_G G)):
+  propagated G S ≡₁ ∅.
+Proof using. unfold propagated. split; basic_solver. Qed. 
+
+Lemma covered_only_cover M
+      (COV: M ⊆₁ action ↓₁ eq ta_cover):
+  covered M ≡₁ event ↑₁ M. 
+Proof using. 
+  unfold covered. split; [basic_solver| ].
+  apply set_collect_mori; auto. generalize COV. basic_solver. 
+Qed. 
+
+Lemma issued_only_issue M
+      (ISS: M ⊆₁ action ↓₁ eq ta_issue):
+  issued M ≡₁ event ↑₁ M. 
+Proof using. 
+  unfold issued. split; [basic_solver| ].
+  apply set_collect_mori; auto. generalize ISS. basic_solver. 
+Qed. 
+
+Lemma reserved_only_reserve M
+      (RES: M ⊆₁ action ↓₁ eq ta_reserve):
+  reserved M ≡₁ event ↑₁ M. 
+Proof using. 
+  unfold reserved. split; [basic_solver| ].
+  apply set_collect_mori; auto. generalize RES. basic_solver. 
+Qed. 
+
+Lemma propagated_only_propagate G (M: trav_label -> Prop)
+      (PROP: M ⊆₁ action ↓₁ is_ta_propagate_to_G G):
+  propagated G M ≡₁ event ↑₁ M. 
+Proof using. 
+  unfold propagated. split; [basic_solver| ].
+  apply set_collect_mori; auto. generalize PROP. basic_solver.
+Qed. 
+
+End SimplificationsCIRP. 
+
+
+
+
+(* The idea for these tactics is to simplify as much terms as possible,
+   leaving those that give unsolved premises as is *)
+(* TODO: is there a better way to do this? *)
+Ltac remember_tls_sets :=
+  repeat (match goal with
+          |  |- context [ (covered ?S) ] => remember (@covered S) eqn:?HeqS
+          |  |- context [ (issued ?S) ] => remember (@issued S) eqn:?HeqS
+          |  |- context [ (reserved ?S) ] => remember (@reserved S) eqn:?HeqS
+          |  |- context [ (propagated ?G ?S) ] => remember (@propagated G S) eqn:?HeqS
+          end).
+
+
+Ltac tls_set_simpl_solvers :=
+  basic_solver 10 || iord_dom_solver || (unfolder; ins; congruence). 
+
+Ltac try_simplify_set nonset_lem only_lem :=
+  try (
+      (rewrite nonset_lem; [| tls_set_simpl_solvers]) ||
+      (rewrite only_lem; [| tls_set_simpl_solvers])
+    ). 
+
+Ltac subst_tls_sets_simpl :=
+  repeat (match goal with
+          | H: ?E = covered ?S |- _ => subst E; try_simplify_set covered_noncover_empty covered_only_cover
+          | H: ?E = issued ?S |- _ => subst E; try_simplify_set issued_nonissue_empty issued_only_issue
+          | H: ?E = reserved ?S |- _ =>
+              subst E; try_simplify_set reserved_nonreserve_empty reserved_only_reserve
+          | H: ?E = propagated ?G ?S |- _ =>
+              subst E; try_simplify_set propagated_nonpropagated_empty propagated_only_propagate
+            end;
+          try rewrite !set_pair_cancel_action
+         ).
+  
+(* TODO: for some reason adding 'set_map_empty' here causes autorewrite to hang.
+   The same behavior occurs with the manual 'repeat'-based implementation. *)
+Create HintDb set_simpl_db.
+Global Hint Rewrite
+       set_union_empty_l set_union_empty_r set_inter_empty_l set_inter_empty_r
+       set_compl_full set_minusK set_compl_empty
+       dom_empty codom_empty eqv_empty
+       set_collect_empty
+  (* set_map_empty *)
+  : set_simpl_db. 
+Ltac simpl_sets := autorewrite with set_simpl_db.
+
+
+Create HintDb tls_sets_simpl_db.
+Global Hint Rewrite
+       covered_union covered_inter covered_minus
+       issued_union issued_inter issued_minus
+       reserved_union reserved_inter reserved_minus
+       propagated_union
+       covered_singleton issued_singleton reserved_singleton
+  : tls_sets_simpl_db. 
+
+Ltac simplify_tls_events :=
+  autorewrite with tls_sets_simpl_db;
+  remember_tls_sets; subst_tls_sets_simpl;
+  simpl_sets. 
+
+Tactic Notation "simplify_tls_events'" :=
+  eapply set_equiv_exp; [by simplify_tls_events| ].
+Tactic Notation "simplify_tls_events'" "in" hyp(H) :=
+  eapply set_equiv_exp in H; [| by simplify_tls_events].
+
+Ltac find_event_set :=
+  eapply set_equiv_exp; [by simplify_tls_events| basic_solver]. 
+
+Ltac separate_set_event :=
+  apply set_disjoint_eq_r; simplify_tls_events; basic_solver. 
+
+
+(* TODO: the problem is that 'autorewrite' either tries to rewrite every occurence, including those with unsatisfiable premises, or (with 'using' clause) stops on first failed rewrite. *)
+(* Create HintDb tls_events_db. *)
+(* Hint Rewrite reserved_union reserved_nonreserve_empty reserved_only_reserve using (basic_solver 10 || iord_dom_solver): tls_events_db. *)
+(* Ltac simplify_tls_events' := autorewrite * with tls_events_db.  *)
+
+Section TacticTest.
+Let test T e:
+  reserved (T ∪₁ eq (mkTL ta_issue e) ∪₁ eq (mkTL ta_reserve e)) ≡₁
+  reserved T ∪₁ eq e.
+Proof using.
+  (* simplify_tls_events'. *)
+  simplify_tls_events.
+  basic_solver. 
+Qed.
+End TacticTest.
+
+Section WfSets.
+  Context (G: execution) (sc: relation actid) (WF: Wf G). 
+  Context
+    (T : trav_label -> Prop)
+    (TLSCOH  : tls_coherent G T)
+    (IORDCOH : iord_coherent G sc T).
+  
+  Notation "'E'" := (acts_set G).
+  Notation "'W'" := (fun x => is_true (is_w (lab G) x)).
+
+  Lemma issuedW :
+    issued T ⊆₁ W.
+  Proof using WF TLSCOH. 
+    unfold issued. rewrite tlsc_I_in_W; eauto. basic_solver.  
+  Qed. 
+
+  Lemma propagatedEW : propagated G T ⊆₁ E ∩₁ W.
+  Proof using WF TLSCOH.
+    clear -WF TLSCOH.
+    unfold propagated.
+    unfolder. ins. desf.
+    unfold is_ta_propagate_to_G in *.
+    unfolder in *. desf.
+    split; [eapply tlsc_P_in_E|eapply tlsc_P_in_W].
+    all: eauto.
+    all: basic_solver.
+  Qed. 
+
+  Lemma propagatedE : propagated G T ⊆₁ E.
+  Proof using WF TLSCOH. rewrite propagatedEW. basic_solver 1. Qed. 
+  Lemma propagatedW : propagated G T ⊆₁ W.
+  Proof using WF TLSCOH. rewrite propagatedEW. basic_solver 1. Qed. 
+
+  Lemma issuedE :
+    issued T ⊆₁ E.
+  Proof using WF TLSCOH.
+    unfold issued. rewrite (tlsc_E WF TLSCOH). basic_solver.  
+  Qed. 
+
+  Lemma coveredE:
+    covered T ⊆₁ E.
+  Proof using WF TLSCOH.
+    unfold covered. rewrite (tlsc_E WF TLSCOH). basic_solver.
+  Qed. 
+
+  Lemma w_covered_issued :
+    W ∩₁ covered T ⊆₁ issued T.
+  Proof using TLSCOH IORDCOH.
+    unfold covered.
+    unfolder. ins. desc.
+    forward eapply tlsc_w_covered_issued with (x := mkTL ta_cover x); eauto.
+    destruct y; ins; vauto. 
+  Qed.
+  
+  Lemma IPROP_in_iord_simpl : IPROP G ⊆ iord_simpl G sc.
+  Proof using. unfold iord_simpl. eauto with hahn. Qed.
+  
+  Lemma init_issued : is_init ∩₁ E ⊆₁ issued T.
+  Proof using TLSCOH.
+    unfolder; ins; desf. red.
+    exists (mkTL ta_issue x). repeat split; auto. 
+    destruct TLSCOH. apply tls_coh_init. red. split; basic_solver. 
+  Qed. 
+
+  Lemma init_covered : is_init ∩₁ E ⊆₁ covered T.
+  Proof using TLSCOH. 
+    unfolder; ins; desf. red.
+    exists (mkTL ta_cover x). repeat split; auto. 
+    destruct TLSCOH. apply tls_coh_init. red. split; basic_solver. 
+  Qed.
+
+  Lemma init_propagated_thread t (Gt: (threads_set G \₁ eq tid_init) t):
+    is_init ∩₁ E ⊆₁ event ↑₁ (T ∩₁ action ↓₁ eq (ta_propagate t)). 
+  Proof using TLSCOH. 
+    unfolder; ins; desf.
+    exists (mkTL (ta_propagate t) x). repeat split; auto. 
+    destruct TLSCOH. apply tls_coh_init. red. split; try basic_solver.
+    right. red. exists t. split; auto.
+  Qed.
+
+  Lemma propagated_in_issued : propagated G T ⊆₁ issued T.
+  Proof using WF TLSCOH IORDCOH.
+    rewrite AuxRel2.set_split_complete with (s' := propagated G T) (s := fun x => is_init x = true).
+    unionL.
+    { rewrite propagatedE. rewrite <- init_issued. clear; basic_solver 1. }
+    arewrite (propagated G T ⊆₁ propagated G T ∩₁ (E ∩₁ W)).
+    { apply set_subset_inter_r. splits; auto.
+      apply propagatedEW. }
+    rewrite <- set_minusE. 
+    rewrite <- set_inter_minus_r.
+    intros x [HH BB]. destruct HH as [[t e] HH]; desf; ins.
+    destruct HH as [HH AA].
+    unfolder in AA; ins.
+    exists (ta_issue, e); ins.
+    splits; auto.
+    split.
+    2: basic_solver 1. 
+    eapply IORDCOH.
+    red. exists (t, e).
+    apply seq_eqv_r. split; auto.
+    do 2 red. splits.
+    all: try now red; ins; generalize BB; clear; basic_solver 10.
+    apply IPROP_in_iord_simpl.
+    red. unfolder; ins. splits; eauto.
+    eexists; splits; eauto.
+    generalize BB; clear; basic_solver 10.
+  Qed.
+
+  Lemma covered_in_coverable: 
+    covered T ⊆₁ coverable G sc T.
+  Proof using WF TLSCOH IORDCOH. 
+    unfold covered, coverable. apply set_subset_inter_r. split; [apply coveredE|].
+    apply set_collect_mori; [done| ]. apply set_subset_inter; [| done].
+    by apply dom_rel_to_cond.
+  Qed.
+
+  Lemma issued_in_issuable:
+    issued T ⊆₁ issuable G sc T.
+  Proof using WF TLSCOH IORDCOH. 
+    unfold issued, issuable. repeat (apply set_subset_inter_r; split); auto using issuedE, issuedW. 
+    apply set_collect_mori; [done| ]. apply set_subset_inter; [| done].
+    by apply dom_rel_to_cond.
+  Qed.
+
+  Lemma issuableE:
+    issuable G sc T ⊆₁ acts_set G. 
+  Proof using. unfold issuable. basic_solver. Qed. 
+  
+  Lemma issuableW:
+    issuable G sc T ⊆₁ is_w (lab G).
+  Proof using. unfold issuable. basic_solver. Qed. 
+
+  Lemma w_coverable_issued :
+    W ∩₁ coverable G sc T ⊆₁ issued T.
+  Proof using TLSCOH.
+    rewrite AuxRel2.set_split_complete with (s' := _ ∩₁ _) (s := is_init).
+    apply set_subset_union_l. split.
+    { rewrite <- init_issued. unfold coverable. basic_solver. } 
+    rewrite <- dom_eqv with (d := _ ∩₁ _). rewrite id_inter, seq_eqvC. 
+    unfold coverable, issued. rewrite !id_inter, <- !seqA. 
+    eapply dom_rel_iord_ext_parts.
+    3: by apply init_issued.
+    2: basic_solver. 
+    transitivity (RF G); [| unfold iord_simpl; basic_solver 10].
+    unfold RF. hahn_frame. basic_solver 10. 
+  Qed.
+
+  Lemma issued_EW :
+    issued T ⊆₁ E ∩₁ W.
+  Proof using WF TLSCOH.
+    unfold issued.
+    apply set_subset_inter_r. split.
+    { apply issuedE; auto. }
+    apply issuedW; auto.
+  Qed.
+
+End WfSets. 
+
+Lemma coverable_iord_dom_cond G sc T e (COV: coverable G sc T e):
+  dom_cond (iord G sc) T (mkTL ta_cover e).
+Proof using. 
+  red in COV. apply proj2 in COV as [[a e_] [[AA [=]] [=]]]. by subst. 
+Qed. 
+
+Lemma issuable_iord_dom_cond G sc T e (ISS: issuable G sc T e):
+  dom_cond (iord G sc) T (mkTL ta_issue e).
+Proof using. 
+  red in ISS. apply proj2 in ISS as [[a e_] [[AA [=]] [=]]]. by subst. 
+Qed. 
