src/travorder/TlsViewRelHelpers.v
@@ -1,0 +1,782 @@
+From hahn Require Import Hahn.
+From PromisingLib Require Import Basic DenseOrder Loc.
+
+From imm Require Import Events.
+From imm Require Import Execution.
+From imm Require Import imm_s.
+From imm Require Import imm_s_hb.
+From imm Require Import imm_bob imm_s_ppo.
+From imm Require Import CombRelations.
+From imm Require Import CombRelationsMore.
+(* Require Import TraversalConfig. *)
+From imm Require Import TraversalOrder. 
+From imm Require Import TLSCoherency.
+From imm Require Import IordCoherency.
+From imm Require Import SimClosure.
+Require Import TlsEventSets.
+Require Import Next. 
+Require Import EventsTraversalOrder.
+
+
+Set Implicit Arguments.
+
+Section ViewRelHelpers.
+
+Variable G : execution.
+Variable WF : Wf G.
+Variable sc : relation actid.
+Variable IMMCON : imm_consistent G sc.
+
+Notation "'co'" := (co G).
+Notation "'sw'" := (sw G).
+Notation "'hb'" := (hb G).
+Notation "'sb'" := (sb G).
+Notation "'rf'" := (rf G).
+Notation "'rfi'" := (rfi G).
+Notation "'rfe'" := (rfe G).
+Notation "'rmw'" := (rmw G).
+Notation "'lab'" := (lab G).
+Notation "'release'" := (release G).
+
+Notation "'Init'" := (fun a => is_true (is_init a)).
+Notation "'E'" := (acts_set G).
+Notation "'R'" := (fun a => is_true (is_r lab a)).
+Notation "'W'" := (fun a => is_true (is_w lab a)).
+Notation "'W_ex'" := (W_ex G).
+Notation "'F'" := (fun a => is_true (is_f lab a)).
+Notation "'Loc_' l" := (fun x => loc lab x = Some l) (at level 1).
+Notation "'Tid_' t" := (fun x => tid x = t) (at level 1).
+Notation "'W_' l" := (W ∩₁ Loc_ l) (at level 1).
+
+Notation "'Pln'" := (fun a => is_true (is_only_pln lab a)).
+Notation "'Rlx'" := (fun a => is_true (is_rlx lab a)).
+Notation "'Rel'" := (fun a => is_true (is_rel lab a)).
+Notation "'Acq'" := (fun a => is_true (is_acq lab a)).
+Notation "'Acqrel'" := (fun a => is_true (is_acqrel lab a)).
+Notation "'Sc'" := (fun a => is_true (is_sc lab a)).
+
+Context
+  (T : trav_label -> Prop)
+  (TLSCOH  : tls_coherent G T)
+  (IORDCOH : iord_coherent G sc T). 
+
+Lemma msg_rel_co_irr l :
+  irreflexive (msg_rel G sc l ⨾ co).
+Proof using WF IMMCON.
+  unfold msg_rel.
+  intros x AA.
+  destruct AA as [y [[z [AA BB]] CC]].
+  eapply release_co_urr_irr; eauto.
+  1-4: by apply IMMCON.
+  eexists; split; [|eexists]; eauto.
+Qed.
+
+
+Lemma s_tm_cov_sc_fence
+      f ordf thread
+      (TID: tid f = thread)
+      (RELCOV : W ∩₁ Rel ∩₁ issued T ⊆₁ covered T)
+      (NEXT : next G (covered T) f)
+      (FPARAMS : lab f = Afence ordf)
+      (SC : Sc f) :
+  forall l,
+    S_tm G l (covered T ∪₁ eq f) ≡₁
+    S_tm G l (covered T) ∪₁ t_acq G sc thread l (covered T).
+Proof using WF TLSCOH IORDCOH IMMCON.
+  cdes IMMCON.
+  intro l; split.
+  - unfold S_tm, t_acq.
+    rewrite s_tmr_union; relsf; unionL; splits; [basic_solver|].
+    unionR right.
+    rewrite (s_tmr_helper _ _ WF).
+    unfold c_acq, urr.
+    arewrite (sb ⨾ ⦗F ∩₁ Sc⦘ ⨾ ⦗eq f⦘ ⊆ ⦗covered T⦘ ⨾ sb ⨾ ⦗eq f⦘).
+      by revert NEXT; unfold next, dom_cond; basic_solver 21.
+    arewrite (⦗covered T⦘ ⨾ sb ⨾ ⦗eq f⦘ ⊆ ⦗Tid_ thread ∪₁ Init⦘ ⨾ ⦗covered T⦘ ⨾ sb^?).
+      by unfolder; ins; desf; splits; eauto using sb_tid_init.
+    basic_solver 42.
+  - unionL; [by unfold S_tm; rewrite s_tmr_union; basic_solver|].
+  unfold t_acq, S_tm.
+  rewrite s_tmr_union.
+  relsf.
+  unfold c_acq, urr.
+  rewrite (crE sc); relsf; unionL; splits.
+  { unionR right.
+    rewrite (s_tmr_helper _ _ WF).
+    arewrite (⦗Tid_ thread ∪₁ Init⦘ ⨾ ⦗covered T⦘ ⊆ ⦗dom_rel(sb ⨾ ⦗eq f⦘)⦘).
+    { rewrite <- TID; rewrite next_helper'; eauto. basic_solver. }
+    arewrite (⦗eq f⦘ ⊆ ⦗F ∩₁ Sc⦘ ⨾ ⦗eq f⦘) at 1 by type_solver.
+    basic_solver 42. }
+  arewrite (⦗Tid_ thread ∪₁ Init⦘ ⨾ ⦗covered T⦘ ⊆ ⦗covered T⦘ ⨾ ⦗Tid_ thread ∪₁ Init⦘).
+  basic_solver.
+
+  arewrite ((release ⨾ rf)^? ⨾ ⦗covered T⦘ ⊆ ⦗covered T⦘ ⨾ (release ⨾ rf)^?).
+  { by case_refl _;
+      [basic_solver| rewrite !seqA; rewrite release_rf_covered; auto; basic_solver]. }
+  arewrite (hb^? ⨾ ⦗covered T⦘ ⊆ ⦗covered T⦘ ⨾ hb^?).
+  { by case_refl _; [basic_solver| rewrite hb_covered; auto; basic_solver]. }
+  arewrite (⦗W_ l⦘ ⨾ rf^? ⨾ (hb ⨾ ⦗F ∩₁ Sc⦘)^? ⨾ sc ⊆ ⦗W_ l⦘ ⨾ rf^? ⨾ hb ⨾ ⦗F ∩₁ Sc⦘ ⨾ sc).
+  rewrite (dom_l (@wf_scD G sc Wf_sc)) at 1; rewrite (dom_r (wf_rfD WF)) at 1; hahn_frame_r; type_solver 42.
+
+  arewrite (sc ⨾ ⦗covered T⦘ ⊆ ⦗covered T⦘ ⨾ sc).
+  { now eapply sc_covered; eauto. }
+  unfold S_tmr; basic_solver 21.
+Qed.
+
+
+Lemma msg_rel_alt
+      (Wf_sc : wf_sc G sc)
+      w (WW : W w) (NCOV : ~ covered T w) (ISS : issuable G sc T w)
+      locw (LOC : loc lab w = Some locw) l:
+  dom_rel (msg_rel G sc l ⨾ ⦗ eq w ⦘) ≡₁
+  (if is_rel lab w
+   then t_cur G sc (tid w) l (covered T ∪₁ eq w)
+   else t_rel G sc (tid w) l locw (covered T)) ∪₁
+  dom_rel (msg_rel G sc l ⨾ (rf ⨾ rmw) ⨾ ⦗ eq w ⦘).
+Proof using WF TLSCOH IORDCOH IMMCON.
+  assert (E w) as EW.
+  { apply ISS. }
+  assert (~ is_init w) as WNIT.
+  { intros H. apply NCOV. eapply init_covered; vauto. }
+
+  assert (Rel w -> dom_rel (sb ⨾ ⦗eq w⦘) ≡₁ (Tid_ (tid w) ∪₁ Init) ∩₁ covered T) as TT.
+  { intros REL. split.
+    { intros x [y H]. apply seq_eqv_r in H; desf.
+      split.
+      { by destruct (sb_tid_init H); [left|right]. }
+
+      eapply fwbob_issuable_in_C; eauto. eexists. apply seq_eqv_r. split; eauto.
+      apply sb_to_w_rel_in_fwbob. apply seq_eqv_r. split; vauto. }
+    intros x [TIDIN COV]. exists w.
+    apply seq_eqv_r; split; auto.
+    assert (E x) as EX by (eapply coveredE; eauto).
+    destruct TIDIN as [TID|INIT].
+    2: by eapply init_ninit_sb; eauto.
+    edestruct same_thread as [H|H].
+    3: by apply WNIT.
+    { apply ISS. }
+    { apply EX. }
+    1,3: done.
+    exfalso.
+    destruct H as [|H]; [by desf|].
+    apply NCOV.
+    eapply dom_sb_covered; eauto. eexists. apply seq_eqv_r. split; eauto. }
+  assert (Rel w -> dom_rel (sb ⨾ ⦗eq w⦘) ⊆₁ covered T) as TT'.
+  { intros H. rewrite (TT H). basic_solver. }
+
+  assert (~ Rel w ->
+          ⦗Rel⦘ ⨾ fwbob G ⨾ ⦗eq w⦘ ⊆
+          ⦗Rel⦘ ⨾ ⦗W_ locw ∪₁ F⦘ ⨾ ⦗Tid_ (tid w) ∪₁ Init⦘ ⨾ ⦗covered T⦘ ⨾ sb ⨾ ⦗eq w⦘) as QQ.
+  { intros HH.
+    arewrite (fwbob G ⨾ ⦗eq w⦘ ⊆ ⦗covered T⦘ ⨾ fwbob G ⨾ ⦗eq w⦘).
+    { intros x y H. apply seq_eqv_l; split; [|done].
+      apply seq_eqv_r in H. desc. subst. 
+      eapply fwbob_issuable_in_C; eauto. eexists. apply seq_eqv_r. split; eauto. }
+    unfold fwbob; rewrite !seq_union_l. rewrite !seqA.
+    arewrite (⦗W ∩₁ Rel⦘ ⨾ ⦗eq w⦘ ⊆ ∅₂) by basic_solver.
+    arewrite (⦗F ∩₁ (fun a : actid => is_ra lab a)⦘ ⨾ ⦗eq w⦘ ⊆ ∅₂) by type_solver.
+    relsf; unionL.
+    - unfold same_loc; unfolder; ins; desf; splits; eauto.
+      by left; splits; congruence.
+      by apply (@sb_tid_init G).
+    - generalize (@sb_tid_init G).
+      basic_solver 21. }
+
+  unfold msg_rel at 1.
+  unfold imm_s_hb.release.
+  unfold imm_s_hb.rs.
+  rewrite rtE.
+  rewrite !seq_union_r. rewrite seq_union_l.
+  rewrite dom_union. apply set_equiv_union.
+  2: { apply dom_rel_more.
+       unfold msg_rel at 1. unfold imm_s_hb.release. unfold imm_s_hb.rs.
+       rewrite ct_end. basic_solver. }
+  rewrite seq_id_r.
+  unfold t_cur, t_rel.
+  split.
+  { rewrite !seqA.
+    arewrite (⦗Rel⦘ ⨾ (⦗F⦘ ⨾ sb)^? ⨾ ⦗W⦘ ⨾ (sb ∩ same_loc lab)^? ⨾ ⦗W⦘ ⨾ ⦗eq w⦘ ⊆
+              ⦗Rel⦘ ⨾ fwbob G ⨾ ⦗eq w⦘ ∪ ⦗Rel ∩₁ eq w⦘).
+    { case_refl _; case_refl _.
+      { basic_solver. }
+      all: unfold fwbob.
+      { basic_solver 42. }
+      all: arewrite (⦗Rel⦘ ⨾ ⦗F⦘ ⊆ ⦗Rel⦘ ⨾ ⦗F ∩₁ (fun a => is_ra lab a)⦘) by mode_solver.
+      2: arewrite (sb ⨾ ⦗W⦘ ⨾ sb ∩ same_loc lab ⊆ sb) by
+          (generalize (@sb_trans G); basic_solver).
+      all: basic_solver 42. }
+    rewrite seq_union_r.
+    desf.
+    { arewrite (Rel ∩₁ eq w ≡₁ eq w); [basic_solver|].
+      arewrite (urr G sc l ⨾ ⦗Rel⦘ ⨾ fwbob G ⨾ ⦗eq w⦘ ∪ urr G sc l ⨾ ⦗eq w⦘ ⊆
+                urr G sc l ⨾ ⦗eq w⦘).
+      { rewrite union_absorb_l; [done|].
+        hahn_frame. etransitivity.
+        2: by apply urr_hb.
+        hahn_frame.
+        rewrite fwbob_in_bob. rewrite bob_in_sb.
+        rewrite sb_in_hb. basic_solver. }
+      rewrite urr_w_alt_union_eqv; auto.
+      apply dom_rel_mori.
+      arewrite (⦗eq w⦘ ⊆ ⦗W⦘ ⨾ ⦗eq w⦘) at 1 by basic_solver.
+      seq_rewrite (urr_w WF); relsf; unionL; [unionR left| basic_solver 12].
+      generalize (TT' Heq); basic_solver 21. }
+    arewrite (Rel ∩₁ eq w ≡₁ ∅) by basic_solver.
+    rewrite <- dom_rel_ext with
+        (r := c_rel G sc (tid w) l locw (covered T))
+        (r' := (sb ⨾ ⦗ eq w ⦘) ).
+    apply dom_rel_mori.
+    unfold c_rel.
+    rewrite crE. rewrite !seq_union_r. unionR right.
+    rewrite !seqA; rewrite QQ; [basic_solver 12| by rewrite Heq]. }
+  desf.
+  { rewrite urr_w_alt_union_eqv; auto.
+    relsf; unionL; splits; [|unfold urr; basic_solver 42].
+    rewrite crE at 1; relsf; unionL; splits.
+    - rewrite seq_eqvC; rewrite <- id_inter.
+      rewrite <- (TT Heq).
+      rewrite dom_rel_eqv_dom_rel.
+      apply dom_rel_mori.
+      rewrite !crE; relsf.
+      unionR left -> left. rewrite !seqA.
+      arewrite (⦗eq w⦘ ⊆ ⦗Rel⦘ ⨾ ⦗eq w⦘) at 1 by basic_solver.
+      arewrite (⦗eq w⦘ ⊆ ⦗W⦘ ⨾ ⦗eq w⦘) at 1 by basic_solver.
+      hahn_frame. etransitivity;[|by apply urr_hb].
+      rewrite sb_in_hb. basic_solver.
+    - rewrite sb_in_hb at 1.
+      arewrite (hb ⊆ hb^?) at 1 .
+      arewrite_id ⦗covered T⦘; rels.
+      sin_rewrite (@urr_hb G sc l).
+      basic_solver 21. }
+  unfold c_rel.
+  rewrite <- !id_inter.
+  intros x [y [z [HH [H'' JJ]]]]; subst.
+  exists w. apply seq_eqv_r; split; auto.
+  exists y; split; auto.
+  destruct JJ as [JJ1 [JJ2 [JJ3 JJ4]]].
+  assert (E y) as EY by (eapply coveredE; eauto). 
+  assert (sb y w) as SBYW.
+  { destruct JJ3 as [TID|INIT].
+    2: by eapply init_ninit_sb; eauto.
+    edestruct same_thread as [H|H].
+    3: by apply WNIT.
+    { apply ISS. }
+    { apply EY. }
+    1,3: done.
+    exfalso.
+    destruct H as [|H]; [by desf|].
+    apply NCOV.
+    eapply dom_sb_covered; eauto. eexists. apply seq_eqv_r. split; eauto. }
+  apply seq_eqv_l; split; auto.
+  destruct JJ2.
+  { exists y; split; [by left|].
+    apply seq_eqv_l; split; [apply H|].
+    apply seq_eqv_r; split; auto.
+    right; split; auto. red. rewrite LOC; apply H. }
+  basic_solver 12.
+Qed.
+
+Lemma msg_rel_alt2
+      (Wf_sc : wf_sc G sc)
+      w (WW : W w) (NCOV : ~ covered T w) (ISS : issuable G sc T w)
+      locw (LOC : loc lab w = Some locw) l:
+  dom_rel (msg_rel G sc l ⨾ ⦗ eq w ⦘) ≡₁
+  (if is_rel lab w
+   then t_cur G sc (tid w) l (covered T)
+   else t_rel G sc (tid w) l locw (covered T)) ∪₁
+  dom_rel (msg_rel G sc l ⨾ (rf ⨾ rmw) ⨾ ⦗ eq w ⦘) ∪₁
+  Rel ∩₁ Loc_ l ∩₁ eq w.
+Proof using WF TLSCOH IORDCOH IMMCON.
+  rewrite msg_rel_alt; eauto.
+  desf.
+  2: by arewrite (Rel ∩₁ Loc_ l ∩₁ eq w ≡₁ ∅); basic_solver 10. 
+  rewrite t_cur_urr_union_eqv_w; auto.
+  { arewrite (Rel ∩₁ Loc_ l ∩₁ eq w ≡₁ Loc_ l ∩₁ eq w).
+    2: by unfold t_cur, c_cur; basic_solver 10.
+    basic_solver 10. }
+  etransitivity; [| apply fwbob_issuable_in_C]; eauto. 
+  generalize (@sb_to_w_rel_in_fwbob G) Heq. basic_solver 10. 
+Qed.
+
+Lemma msg_rel_rfrmw_helper
+      w (WW : W w) (NCOV : ~ covered T w) (ISS : issuable G sc T w)
+      locw (LOC : loc lab w = Some locw) l:
+  dom_rel ((urr G sc l ⨾ release) ⨾ (rf ⨾ rmw) ⨾ ⦗eq w⦘) ⊆₁
+  dom_rel (urr G sc l ⨾ ⦗Rel⦘ ⨾ ⦗W_ locw ∪₁ F⦘ ⨾ ⦗Tid_ (tid w) ∪₁ Init⦘ ⨾ ⦗covered T⦘)
+  ∪₁ dom_rel ((urr G sc l ⨾ release) ⨾ (⦗W_ex⦘ ⨾ rfi ∪ rfe) ⨾ rmw ⨾ ⦗eq w⦘).
+Proof using WF TLSCOH IMMCON.
+rewrite rfi_union_rfe; relsf; unionL; splits.
+2: basic_solver 12.
+unfold imm_s_hb.release.
+unfold imm_s_hb.rs.
+rewrite rtE; relsf.
+unionL; splits; cycle 1.
+rewrite rmw_W_ex at 1.
+rewrite <- !seqA.
+rewrite inclusion_ct_seq_eqv_r.
+unionR right -> left -> right; basic_solver 21.
+unionR left.
+rewrite !seqA.
+arewrite ((sb ∩ same_loc lab)^? ⨾ ⦗W⦘ ⨾ rfi ⨾ rmw ⊆ sb ∩ same_loc lab).
+{ arewrite_id ⦗W⦘; rewrite (rfi_in_sbloc' WF), (rmw_in_sb_loc WF).
+  generalize (@sb_same_loc_trans G); ins; relsf. }
+arewrite (⦗Rel⦘ ⨾ (⦗F⦘ ⨾ sb)^? ⨾ ⦗W⦘ ⨾ sb ∩ same_loc lab ⨾ ⦗eq w⦘
+   ⊆ ⦗Rel⦘ ⨾ ⦗W_ locw ∪₁ F⦘ ⨾ ⦗Tid_ (tid w) ∪₁ Init⦘ ⨾ fwbob G ⨾ ⦗eq w⦘).
+{ 
+rewrite crE at 1; relsf; unionL.
+- unfold fwbob.
+rewrite sb_tid_init' at 1.
+rewrite (init_pln WF) at 1.
+unfold same_tid.
+relsf.
+unionR left -> left -> right.
+unfolder; ins; desf; splits; eauto 20.
+unfold same_loc in *; desf; eauto; left; splits; congruence.
+unfold same_loc in *; desf; eauto; left; splits; congruence.
+mode_solver 42.
+- 
+rewrite !seqA.
+arewrite (sb ⨾ ⦗W⦘ ⨾ sb ∩ same_loc lab ⊆ sb).
+by generalize (@sb_trans G); basic_solver.
+arewrite (⦗Rel⦘ ⨾ ⦗F⦘ ⨾ sb ⨾ ⦗eq w⦘ ⊆ ⦗Rel⦘ ⨾ ⦗F⦘ ⨾ ⦗Tid_ (tid w)⦘ ⨾ fwbob G ⨾ ⦗eq w⦘).
+{ unfold fwbob.
+rewrite sb_tid_init' at 1.
+rewrite (init_w WF).
+unfold same_tid.
+mode_solver 21. }
+basic_solver.
+
+}
+
+arewrite (⦗eq w⦘ ⊆ ⦗dom_cond (fwbob G) (covered T)⦘).
+{ apply eqv_rel_mori. apply set_subset_eq.
+  eapply AuxDef.dom_rel_to_cond; eauto. apply fwbob_issuable_in_C; auto. }
+rewrite dom_cond_elim.
+basic_solver 12.
+Qed.
+
+Lemma t_rel_msg_rel_rfrmw
+      w (WW : W w) (NCOV : ~ covered T w) (ISS : issuable G sc T w)
+      locw (LOC : loc lab w = Some locw) l:
+  t_rel G sc (tid w) l locw (covered T) ∪₁ dom_rel (msg_rel G sc l ⨾ (rf ⨾ rmw) ⨾ ⦗eq w⦘) ≡₁
+  t_rel G sc (tid w) l locw (covered T) ∪₁
+  dom_rel (msg_rel G sc l ⨾ (⦗ W_ex ⦘ ⨾ rfi ∪ rfe) ⨾ rmw ⨾ ⦗eq w⦘).
+Proof using WF TLSCOH IMMCON.
+ins; split; unionL; desf.
+1,3: basic_solver.
+2: rewrite rfi_union_rfe; basic_solver 12.
+unfold t_rel, c_rel, msg_rel.
+by apply msg_rel_rfrmw_helper.
+Qed.
+
+Lemma t_cur_msg_rel_rfrmw
+      w (WW : W w) (NCOV : ~ covered T w) (ISS : issuable G sc T w) l:
+  t_cur G sc (tid w) l (covered T) ∪₁ dom_rel (msg_rel G sc l ⨾ (rf ⨾ rmw) ⨾ ⦗eq w⦘) ≡₁
+  t_cur G sc (tid w) l (covered T) ∪₁
+  dom_rel (msg_rel G sc l ⨾ (⦗ W_ex ⦘ ⨾ rfi ∪ rfe) ⨾ rmw ⨾ ⦗eq w⦘).
+Proof using WF TLSCOH IMMCON.
+ins; split; unionL; desf.
+1,3: basic_solver.
+2: rewrite rfi_union_rfe; basic_solver 12.
+unfold t_cur, c_cur, msg_rel.
+assert (exists locw, loc lab w = Some locw).
+by unfold loc, is_w in *; destruct (lab w); eauto.
+desc.
+rewrite msg_rel_rfrmw_helper; try edone.
+basic_solver 21.
+Qed.
+
+Lemma t_cur_n_sc_fence_step
+      (Wf_sc : wf_sc G sc)
+      f (FENCE : F f) (NSC : ~ Sc f) (NEXT : next G (covered T) f)
+      (RELCOV : W ∩₁ Rel ∩₁ issued T ⊆₁ covered T):
+  forall l,
+    t_cur G sc (tid f) l (covered T ∪₁ eq f) ≡₁
+    if is_acq lab f
+    then t_acq G sc (tid f) l (covered T)
+    else t_cur G sc (tid f) l (covered T).
+Proof using WF TLSCOH IORDCOH IMMCON.
+ins; split; rewrite t_cur_union; unionL; desf.
+by apply t_cur_in_t_acq.
+4: basic_solver.
+all: unfold t_cur, t_acq, c_cur, c_acq.
+- arewrite (⦗Tid_ (tid f) ∪₁ Init⦘ ⨾ ⦗eq f⦘ ⊆ ⦗eq f⦘ ⨾ ⦗Tid_ (tid f) ∪₁ Init⦘) by basic_solver.
+  arewrite (⦗eq f⦘ ⊆ ⦗ F ∩₁ set_compl Sc ⦘ ⨾ ⦗eq f⦘) by basic_solver.
+  sin_rewrite (urr_f_non_sc WF); auto.
+  rewrite next_helper'; basic_solver 21.
+- arewrite (⦗Tid_ (tid f) ∪₁ Init⦘ ⨾ ⦗eq f⦘ ⊆ ⦗eq f⦘ ⨾ ⦗Tid_ (tid f) ∪₁ Init⦘) by basic_solver.
+  arewrite (⦗eq f⦘ ⊆ ⦗ F∩₁set_compl Acq ⦘ ⨾ ⦗eq f⦘) by basic_solver.
+  sin_rewrite (urr_f_non_acq WF); auto.
+  rewrite next_helper'; basic_solver 21.
+- rewrite crE at 1; relsf; unionL; splits; [basic_solver 12|].
+  unionR right.
+  rewrite next_helper'; eauto.
+  rewrite <- !seqA.
+  rewrite !dom_rel_eqv_dom_rel.
+  rewrite !seqA.
+  arewrite (⦗eq f⦘ ⊆ ⦗ F∩₁ Acq ⦘ ⨾ ⦗eq f⦘) at 1 by basic_solver.
+  arewrite (release ⨾ rf ⨾ sb ⨾ ⦗F ∩₁ Acq⦘ ⊆ sw).
+  unfold imm_s_hb.sw; basic_solver 16.
+  arewrite (sw ⊆ hb^?).
+  sin_rewrite urr_hb.
+  basic_solver 21.
+Qed.
+
+Lemma t_acq_n_sc_fence_step
+      (Wf_sc : wf_sc G sc)
+      f (FENCE : F f) (NSC : ~ Sc f) (NEXT : next G (covered T) f):
+  forall l,
+    t_acq G sc (tid f) l (covered T ∪₁ eq f) ≡₁
+    t_acq G sc (tid f) l (covered T).
+Proof using WF TLSCOH IORDCOH IMMCON.
+ins; split; rewrite t_acq_union; unionL; splits; desf; [|basic_solver].
+unfold t_acq, c_acq.
+arewrite (⦗Tid_ (tid f) ∪₁ Init⦘ ⨾ ⦗eq f⦘ ⊆ ⦗eq f⦘ ⨾ ⦗Tid_ (tid f) ∪₁ Init⦘) by basic_solver.
+rewrite next_helper'; eauto.
+rewrite <- !seqA.
+rewrite !dom_rel_eqv_dom_rel.
+rewrite !seqA.
+rewrite (dom_r (wf_rfD WF)) at 1.
+rewrite crE at 1; relsf; unionL; splits; [|type_solver].
+arewrite (⦗eq f⦘ ⊆ ⦗ F∩₁set_compl Sc ⦘ ⨾ ⦗eq f⦘) at 1 by basic_solver.
+sin_rewrite (urr_f_non_sc WF); auto.
+basic_solver 21.
+Qed.
+
+Lemma t_rel_n_sc_fence_step
+      (Wf_sc : wf_sc G sc)
+      f (FENCE : F f) (NSC : ~ Sc f) (NEXT : next G (covered T) f):
+  forall l l',
+    t_rel G sc (tid f) l l' (covered T ∪₁ eq f) ∪₁
+    (if LocSet.Facts.eq_dec l l'
+     then W ∩₁ Loc_ l' ∩₁ Tid_ (tid f) ∩₁ (covered T ∪₁ eq f)
+     else ∅) ≡₁
+    if is_acqrel lab f
+    then t_acq G sc (tid f) l (covered T)
+    else
+      if is_rel lab f
+      then t_cur G sc (tid f) l (covered T)
+      else
+        t_rel G sc (tid f) l l' (covered T) ∪₁
+        (if LocSet.Facts.eq_dec l l'
+         then W ∩₁ Loc_ l' ∩₁ Tid_ (tid f) ∩₁ (covered T)
+         else ∅).
+Proof using WF TLSCOH IORDCOH IMMCON.
+ins; split; try rewrite t_rel_union; unionL; desf.
+by apply t_rel_in_t_acq.
+by apply t_rel_in_t_cur.
+all: try rewrite set_inter_union_r.
+all: unionL.
+all: try  basic_solver 8.
+all: try type_solver.
+5: unfold t_acq, c_acq, urr; basic_solver 42.
+5: unfold t_cur, c_cur, urr; basic_solver 42.
+all: try rewrite set_union_empty_r.
+all: unfold t_rel, c_rel, t_acq, c_acq, t_cur, c_cur.
+all: rewrite next_helper'; eauto.
+all: rewrite <- !seqA, dom_rel_eqv_dom_rel, !seqA.
+- arewrite ( ⦗Rel⦘ ⨾ ⦗W_ l' ∪₁ F⦘ ⨾ ⦗Tid_ (tid f) ∪₁ Init⦘ ⨾ ⦗eq f⦘ ⊆ ⦗F∩₁set_compl Sc⦘ ⨾ ⦗eq f⦘).
+  type_solver.
+  sin_rewrite (urr_f_non_sc WF); auto.
+  basic_solver 21.
+- arewrite ( ⦗Rel⦘ ⨾ ⦗W_ l' ∪₁ F⦘ ⨾ ⦗Tid_ (tid f) ∪₁ Init⦘ ⨾ ⦗eq f⦘ ⊆ ⦗F∩₁set_compl Acq⦘ ⨾ ⦗eq f⦘).
+  mode_solver.
+  sin_rewrite (urr_f_non_acq WF); auto.
+  basic_solver 21.
+- arewrite ( ⦗Rel⦘ ⨾ ⦗W_ l' ∪₁ F⦘ ⨾ ⦗Tid_ (tid f) ∪₁ Init⦘ ⨾ ⦗eq f⦘ ⊆ ⦗F∩₁set_compl Acq⦘ ⨾ ⦗Rel⦘ ⨾ ⦗W_ l' ∪₁ F⦘ ⨾ ⦗eq f⦘).
+  mode_solver.
+  sin_rewrite (urr_f_non_acq WF); auto.
+  basic_solver 21.
+- arewrite ( ⦗Rel⦘ ⨾ ⦗W_ l' ∪₁ F⦘ ⨾ ⦗Tid_ (tid f) ∪₁ Init⦘ ⨾ ⦗eq f⦘ ⊆ ⦗F∩₁set_compl Acq⦘ ⨾ ⦗Rel⦘ ⨾ ⦗W_ l' ∪₁ F⦘ ⨾ ⦗eq f⦘).
+  mode_solver.
+  sin_rewrite (urr_f_non_acq WF); auto.
+  basic_solver 21.
+- arewrite ((release ⨾ rf)^? ⨾ sb ⨾ ⦗eq f⦘ ⊆ hb^? ⨾ ⦗eq f⦘) at 1.
+  { rewrite crE at 1; relsf; unionL.
+    arewrite (sb ⊆ hb^?) at 1; basic_solver.
+    arewrite (⦗eq f⦘ ⊆ ⦗ F∩₁ Acq ⦘ ⨾ ⦗eq f⦘) at 1 by mode_solver.
+    arewrite (release ⨾ rf ⨾ sb ⨾ ⦗F ∩₁ Acq⦘ ⊆ sw).
+    unfold imm_s_hb.sw; basic_solver 16.
+    arewrite (sw ⊆ hb^?); basic_solver. }
+  sin_rewrite urr_hb.
+  arewrite (⦗eq f⦘ ⊆ ⦗ F∩₁ Rel ⦘ ⨾ ⦗eq f⦘) at 1 by mode_solver.
+  basic_solver 21.
+- arewrite ((release ⨾ rf)^? ⨾ sb ⨾ ⦗eq f⦘ ⊆ hb^? ⨾ ⦗eq f⦘) at 1.
+  { rewrite crE at 1; relsf; unionL.
+    arewrite (sb ⊆ hb^?) at 1; basic_solver.
+    arewrite (⦗eq f⦘ ⊆ ⦗ F∩₁ Acq ⦘ ⨾ ⦗eq f⦘) at 1 by mode_solver.
+    arewrite (release ⨾ rf ⨾ sb ⨾ ⦗F ∩₁ Acq⦘ ⊆ sw).
+    unfold imm_s_hb.sw; basic_solver 16.
+    arewrite (sw ⊆ hb^?); basic_solver. }
+  sin_rewrite urr_hb.
+  arewrite (⦗eq f⦘ ⊆ ⦗ F∩₁ Rel ⦘ ⨾ ⦗eq f⦘) at 1 by mode_solver.
+  basic_solver 21.
+- arewrite (sb ⊆ hb^?) at 1.
+  sin_rewrite urr_hb.
+  basic_solver 21.
+- arewrite (sb ⊆ hb^?) at 1.
+  sin_rewrite urr_hb.
+  basic_solver 21.
+Qed.
+
+Lemma sc_helper' (Wf_sc : wf_sc G sc)
+ f (FENCE : F f) (SC : Sc f) (COV : coverable G sc T f) (NCOV : ~ covered T f) :
+ ⦗F ∩₁ Sc⦘ ⨾ ⦗covered T⦘ ≡ ⦗dom_rel (sc ⨾ ⦗eq f⦘)⦘.
+Proof using WF TLSCOH IORDCOH IMMCON.
+split. 
+- unfold coverable, dom_cond in *.
+  unfolder in *; desf; try type_solver. 
+  ins; desf; splits; eauto.
+  eexists; splits; eauto.
+  eapply tot_ex.
+  * apply Wf_sc.
+  * basic_solver.
+  * generalize coveredE; basic_solver.
+  * intro; apply NCOV. eapply dom_sc_covered; vauto.
+  * intro; subst; eauto.
+- rewrite <- !id_inter. apply eqv_rel_mori. apply set_subset_inter_r. split.
+  { rewrite (wf_scD Wf_sc). basic_solver. } 
+  rewrite <- dom_sc_coverable; eauto. basic_solver.  
+Qed.
+
+Lemma coverable_next_covered e
+      (COV: coverable G sc T e)
+      (NCOV : ~ covered T e):
+  next G (covered T) e. 
+Proof using TLSCOH. 
+  red. split; auto. split; [apply COV| ].
+  red. erewrite <- dom_sb_coverable; eauto.
+  basic_solver. 
+Qed. 
+
+Lemma t_cur_sc_fence_step 
+      (RELCOV : W ∩₁ Rel ∩₁ issued T ⊆₁ covered T)
+      f (FENCE : F f) (SC: Sc f) 
+      (COV : coverable G sc T f) (NCOV : ~ covered T f) :
+  forall l,
+    t_cur G sc (tid f) l (covered T ∪₁ eq f) ≡₁
+    S_tm G l (covered T) ∪₁ t_acq G sc (tid f) l (covered T).
+Proof using WF TLSCOH IORDCOH IMMCON.
+  cdes IMMCON.
+ins; split; try rewrite t_cur_union; unionL; desf.
+by rewrite t_cur_in_t_acq; basic_solver.
+all: unfold t_cur, c_cur, S_tm, S_tmr, t_acq, c_acq, t_rel, c_rel.
+- arewrite (⦗Tid_ (tid f) ∪₁ Init⦘ ⨾ ⦗eq f⦘ ⊆ ⦗F ∩₁ Sc⦘ ⨾  ⦗eq f⦘ ⨾ ⦗Tid_ (tid f) ∪₁ Init⦘).
+  basic_solver.
+  sin_rewrite (urr_f_sc WF); auto.
+  rewrite !seqA.
+  arewrite (⦗W_ l⦘ ⨾ rf^? ⨾ (hb ⨾ ⦗F ∩₁ Sc⦘)^? ⨾ sc^? ⨾ ⦗eq f⦘ ⊆ ⦗W_ l⦘ ⨾ rf^? ⨾ hb ⨾ ⦗F ∩₁ Sc⦘ ⨾ sc^? ⨾ ⦗eq f⦘).
+  { rewrite (dom_r (wf_rfD WF)) at 1.
+    arewrite (⦗eq f⦘ ⊆ ⦗F ∩₁ Sc⦘ ⨾  ⦗eq f⦘) at 1 by basic_solver.
+    rewrite (dom_l (wf_scD Wf_sc)) at 1.
+    hahn_frame_r; unfolder; ins; desf; eauto 20; type_solver. }
+  rewrite (crE sc); relsf.
+  rewrite <- !dom_eqv1.
+  unionL; splits.
+  * arewrite (⦗W_ l⦘ ⨾ rf^? ⨾ hb ⨾ ⦗F ∩₁ Sc⦘ ⨾ ⦗eq f⦘ ⊆ S_tmr G l (eq f)).
+    rewrite (s_tmr_helper l (eq f) WF).
+    rewrite next_helper'; eauto using coverable_next_covered.
+    rewrite <- !seqA, dom_rel_eqv_dom_rel, !seqA.
+    unfold urr.
+    unionR right; basic_solver 42.
+  * unfold urr.
+    rewrite (sc_helper' Wf_sc FENCE); auto.
+    basic_solver 21.
+- unfold urr.
+  rewrite (sc_helper' Wf_sc FENCE); auto.
+  rewrite <- !seqA, dom_rel_eqv_dom_rel, !seqA.
+  rewrite (dom_l (wf_scD Wf_sc)) at 1.
+  unionR right; basic_solver 21.
+- rewrite crE at 1; relsf; unionL; splits; [basic_solver 12|].
+  unionR right.
+  rewrite next_helper'; eauto using coverable_next_covered.
+  rewrite <- !seqA.
+  rewrite !dom_rel_eqv_dom_rel.
+  rewrite !seqA.
+  arewrite (⦗eq f⦘ ⊆ ⦗ F∩₁ Acq ⦘ ⨾ ⦗eq f⦘) at 1 by mode_solver.
+  arewrite (release ⨾ rf ⨾ sb ⨾ ⦗F ∩₁ Acq⦘ ⊆ sw).
+  unfold imm_s_hb.sw; basic_solver 16.
+  arewrite (sw ⊆ hb^?).
+  sin_rewrite urr_hb.
+  basic_solver 21.
+Qed.
+
+Lemma t_acq_sc_fence_step
+      f (FENCE : F f) (SC: Sc f) (COV : coverable G sc T f) (NCOV : ~ covered T f):
+  forall l,
+    t_acq G sc (tid f) l (covered T ∪₁ eq f) ≡₁
+    t_acq G sc (tid f) l (covered T) ∪₁
+    S_tm G l (covered T).
+Proof using WF TLSCOH IORDCOH IMMCON.
+  cdes IMMCON.
+ins; split; try rewrite t_acq_union; unionL; desf.
+1,3: basic_solver.
+all: unfold t_cur, c_cur, S_tm, S_tmr, t_acq, c_acq, t_rel, c_rel.
+- arewrite (⦗Tid_ (tid f) ∪₁ Init⦘ ⨾ ⦗eq f⦘ ⊆ ⦗F ∩₁ Sc⦘ ⨾  ⦗eq f⦘ ⨾ ⦗Tid_ (tid f) ∪₁ Init⦘).
+  basic_solver.
+  arewrite ((release ⨾ rf)^? ⨾ ⦗F ∩₁ Sc⦘ ⊆ ⦗F ∩₁ Sc⦘).
+  rewrite (dom_r (wf_rfD WF)) at 1; type_solver.
+  sin_rewrite (urr_f_sc WF); auto.
+  rewrite !seqA.
+  arewrite (⦗W_ l⦘ ⨾ rf^? ⨾ (hb ⨾ ⦗F ∩₁ Sc⦘)^? ⨾ sc^? ⨾ ⦗eq f⦘ ⊆ ⦗W_ l⦘ ⨾ rf^? ⨾ hb ⨾ ⦗F ∩₁ Sc⦘ ⨾ sc^? ⨾ ⦗eq f⦘).
+  { rewrite (dom_r (wf_rfD WF)) at 1.
+    arewrite (⦗eq f⦘ ⊆ ⦗F ∩₁ Sc⦘ ⨾  ⦗eq f⦘) at 1 by basic_solver.
+    rewrite (dom_l (wf_scD Wf_sc)) at 1.
+    hahn_frame_r; unfolder; ins; desf; eauto 20; type_solver. }
+  rewrite (crE sc); relsf; rewrite <- !dom_eqv1; unionL; splits.
+  * arewrite (⦗W_ l⦘ ⨾ rf^? ⨾ hb ⨾ ⦗F ∩₁ Sc⦘ ⨾ ⦗eq f⦘ ⊆ S_tmr G l (eq f)).
+    rewrite (s_tmr_helper l (eq f) WF).
+    rewrite next_helper'; eauto using coverable_next_covered.
+    rewrite <- !seqA, dom_rel_eqv_dom_rel, !seqA.
+    unfold urr.
+    unionR left; basic_solver 42.
+  * unfold urr.
+    rewrite (sc_helper' Wf_sc FENCE); auto.
+    basic_solver 21.
+- unfold urr.
+  rewrite (sc_helper' Wf_sc FENCE); auto.
+  rewrite <- !seqA, dom_rel_eqv_dom_rel, !seqA.
+  rewrite (dom_l (wf_scD Wf_sc)) at 1.
+  unionR right; basic_solver 42.
+Qed.
+
+Lemma t_rel_sc_fence_step
+      f (FENCE : F f) (SC: Sc f) (COV : coverable G sc T f) (NCOV : ~ covered T f) :
+  forall l l',
+    t_rel G sc (tid f) l l' (covered T ∪₁ eq f) ∪₁
+    (if LocSet.Facts.eq_dec l l'
+     then W ∩₁ Loc_ l' ∩₁ Tid_ (tid f) ∩₁ (covered T ∪₁ eq f)
+     else ∅) ≡₁
+     S_tm G l (covered T) ∪₁ t_acq G sc (tid f) l (covered T).
+Proof using WF TLSCOH IORDCOH IMMCON.
+  cdes IMMCON.
+ins; split; try rewrite t_rel_union; unionL; desf.
+by rewrite t_rel_in_t_acq; basic_solver.
+all: unfold t_cur, c_cur, S_tm, S_tmr, t_acq, c_acq, t_rel, c_rel.
+2: by unfold urr; type_solver 42.
+- arewrite (⦗Rel⦘ ⨾ ⦗W_ l' ∪₁ F⦘ ⨾ ⦗Tid_ (tid f) ∪₁ Init⦘ ⨾ ⦗eq f⦘ ⊆ ⦗F ∩₁ Sc⦘ ⨾  ⦗eq f⦘ ⨾ ⦗Tid_ (tid f) ∪₁ Init⦘).
+  basic_solver.
+  sin_rewrite (urr_f_sc WF); auto.
+  rewrite !seqA.
+  arewrite (⦗W_ l⦘ ⨾ rf^? ⨾ (hb ⨾ ⦗F ∩₁ Sc⦘)^? ⨾ sc^? ⨾ ⦗eq f⦘ ⊆ ⦗W_ l⦘ ⨾ rf^? ⨾ hb ⨾ ⦗F ∩₁ Sc⦘ ⨾ sc^? ⨾ ⦗eq f⦘).
+  { rewrite (dom_r (wf_rfD WF)) at 1.
+    arewrite (⦗eq f⦘ ⊆ ⦗F ∩₁ Sc⦘ ⨾  ⦗eq f⦘) at 1 by basic_solver.
+    rewrite (dom_l (wf_scD Wf_sc)) at 1.
+    hahn_frame_r; unfolder; ins; desf; eauto 20; type_solver. }
+  rewrite (crE sc); relsf; rewrite <- !dom_eqv1; unionL; splits.
+  * arewrite (⦗W_ l⦘ ⨾ rf^? ⨾ hb ⨾ ⦗F ∩₁ Sc⦘ ⨾ ⦗eq f⦘ ⊆ S_tmr G l (eq f)).
+    rewrite (s_tmr_helper l (eq f) WF).
+    rewrite next_helper'; eauto using coverable_next_covered.
+    rewrite <- !seqA, dom_rel_eqv_dom_rel, !seqA.
+    unfold urr.
+    unionR right; basic_solver 42.
+  * unfold urr.
+    rewrite (sc_helper' Wf_sc FENCE); auto.
+    basic_solver 21.
+- unfold urr.
+  rewrite (sc_helper' Wf_sc FENCE); auto.
+  rewrite <- !seqA, dom_rel_eqv_dom_rel, !seqA.
+  rewrite (dom_l (wf_scD Wf_sc)) at 1.
+  assert (Rel f) by mode_solver.
+  unionR left -> right; basic_solver 42.
+- unfold urr.
+  rewrite (sc_helper' Wf_sc FENCE); auto.
+  rewrite <- !seqA, dom_rel_eqv_dom_rel, !seqA.
+  rewrite (dom_l (wf_scD Wf_sc)) at 1.
+  assert (Rel f) by mode_solver.
+  unionR left -> right; basic_solver 42.
+- rewrite next_helper'; eauto using coverable_next_covered.
+  rewrite <- !seqA, dom_rel_eqv_dom_rel, !seqA.
+  arewrite ((release ⨾ rf)^? ⨾ sb ⨾ ⦗eq f⦘ ⊆ hb^? ⨾ ⦗eq f⦘) at 1.
+  { rewrite crE at 1; relsf; unionL.
+    arewrite (sb ⊆ hb^?) at 1; basic_solver.
+    arewrite (⦗eq f⦘ ⊆ ⦗ F∩₁ Acq ⦘ ⨾ ⦗eq f⦘) at 1 by mode_solver.
+    arewrite (release ⨾ rf ⨾ sb ⨾ ⦗F ∩₁ Acq⦘ ⊆ sw).
+    unfold imm_s_hb.sw; basic_solver 16.
+    arewrite (sw ⊆ hb^?); basic_solver. }
+  sin_rewrite urr_hb.
+  arewrite (⦗eq f⦘ ⊆ ⦗ F∩₁ Rel ⦘ ⨾ ⦗eq f⦘) at 1 by mode_solver.
+  basic_solver 21.
+- rewrite next_helper'; eauto using coverable_next_covered.
+  rewrite <- !seqA, dom_rel_eqv_dom_rel, !seqA.
+  arewrite ((release ⨾ rf)^? ⨾ sb ⨾ ⦗eq f⦘ ⊆ hb^? ⨾ ⦗eq f⦘) at 1.
+  { rewrite crE at 1; relsf; unionL.
+    arewrite (sb ⊆ hb^?) at 1; basic_solver.
+    arewrite (⦗eq f⦘ ⊆ ⦗ F∩₁ Acq ⦘ ⨾ ⦗eq f⦘) at 1 by mode_solver.
+    arewrite (release ⨾ rf ⨾ sb ⨾ ⦗F ∩₁ Acq⦘ ⊆ sw).
+    unfold imm_s_hb.sw; basic_solver 16.
+    arewrite (sw ⊆ hb^?); basic_solver. }
+  sin_rewrite urr_hb.
+  arewrite (⦗eq f⦘ ⊆ ⦗ F∩₁ Rel ⦘ ⨾ ⦗eq f⦘) at 1 by mode_solver.
+  basic_solver 21.
+Qed.
+
+
+
+Lemma t_cur_fence_step
+      (RELCOV : W ∩₁ Rel ∩₁ issued T ⊆₁ covered T)
+      f (FENCE : F f) (COV : coverable G sc T f) (NCOV : ~ covered T f):
+  forall l,
+    t_cur G sc (tid f) l (covered T ∪₁ eq f) ≡₁
+    if is_sc lab f
+    then S_tm G l (covered T) ∪₁ t_acq G sc (tid f) l (covered T)
+    else
+      if is_acq lab f
+      then t_acq G sc (tid f) l (covered T)
+      else t_cur G sc (tid f) l (covered T).
+Proof using WF TLSCOH IORDCOH IMMCON.
+  destruct (is_sc lab f) eqn: H.
+  apply t_cur_sc_fence_step; auto.
+  apply t_cur_n_sc_fence_step; auto.
+  by apply IMMCON.
+  by ins; desf.
+  apply coverable_next_covered; auto.
+Qed.
+
+Lemma t_acq_fence_step
+      f (FENCE : F f) (COV : coverable G sc T f) (NCOV : ~ covered T f):
+  forall l,
+    t_acq G sc (tid f) l (covered T ∪₁ eq f) ≡₁
+    t_acq G sc (tid f) l (covered T) ∪₁
+    if is_sc lab f
+    then S_tm G l (covered T)
+    else ∅.
+Proof using WF TLSCOH IORDCOH IMMCON.
+  destruct (is_sc lab f) eqn: H.
+  apply t_acq_sc_fence_step; auto.
+  ins; rewrite set_union_empty_r; apply t_acq_n_sc_fence_step; auto.
+  by apply IMMCON.
+  by ins; desf.
+  apply coverable_next_covered; auto.
+Qed.
+
+Lemma t_rel_fence_step
+      f (FENCE : F f) (COV : coverable G sc T f) (NCOV : ~ covered T f) :
+  forall l l',
+    t_rel G sc (tid f) l l' (covered T ∪₁ eq f) ∪₁
+    (if LocSet.Facts.eq_dec l l'
+     then W ∩₁ Loc_ l' ∩₁ Tid_ (tid f) ∩₁ (covered T ∪₁ eq f)
+     else ∅) ≡₁
+    if is_sc lab f
+    then S_tm G l (covered T) ∪₁ t_acq G sc (tid f) l (covered T)
+    else 
+      if is_acqrel lab f
+      then t_acq G sc (tid f) l (covered T)
+      else
+        if is_rel lab f
+        then t_cur G sc (tid f) l (covered T)
+        else
+          (t_rel G sc (tid f) l l' (covered T) ∪₁
+           (if LocSet.Facts.eq_dec l l'
+            then W ∩₁ Loc_ l' ∩₁ Tid_ (tid f) ∩₁ (covered T)
+            else ∅)).
+Proof using WF TLSCOH IORDCOH IMMCON.
+  destruct (is_sc lab f) eqn: H.
+  apply t_rel_sc_fence_step; auto.
+  apply t_rel_n_sc_fence_step; auto.
+  by apply IMMCON.
+  by ins; desf.
+  apply coverable_next_covered; auto. 
+Qed.
+
+End ViewRelHelpers.
